#! https://www.zhihu.com/question/457049386/answer/1860190456

[comment]: <> (Answer URL: https://www.zhihu.com/question/457049386/answer/1860190456)
[comment]: <> "请问这个矩阵的求和是怎么推导的？"
[comment]: <> (Author Name: https://www.zhihu.com/people/quarrying)

问题转化为求证: $\sum_{i=0}^{n} A^i = (A - I)^{-1}(A^{n+1} - I)$

证明如下:

$\sum_{i=0}^{n+1} A^{i} = I + \sum_{i=1}^{n+1} A^{i} = I + A\sum_{i=0}^{n} A^{i}$

$\sum_{i=0}^{n+1} A^{i} = A^{n+1} + \sum_{i=0}^{n} A^{i}$

所以: 

$$
I + A\sum_{i=0}^{n} A^{i} = A^{n+1} + \sum_{i=0}^{n} A^{i} \\
A\sum_{i=0}^{n} A^{i} - \sum_{i=0}^{n} A^{i} = A^{n+1} - I \\
(A - I) \sum_{i=0}^{n} A^{i} = A^{n+1} - I \\
 \sum_{i=0}^{n} A^{i} = (A - I)^{-1}(A^{n+1} - I)
$$
上面推导中假设 $A - I$ 是可逆的.