#! https://zhuanlan.zhihu.com/p/162854898
@title  C/C++之逻辑右移与算术右移


设符号数表示为:  $x = -u_{n-1}2^{n-1} + \sum_{i=0}^{n-2}{u_i2^{i}}$  ,  $u_i \in \{0, 1\}$  (采用 two's complement 编码方式).

逻辑右移, 其中  $k \in \{0, 1, \cdots, n-1\}$  :

$$\begin{aligned}
x \gg_L k 
&= \left\lfloor\left(\sum_{i=0}^{n-1}{u_i2^{i}}\right) / 2^k \right\rfloor 
= \left\lfloor\sum_{i=0}^{n-1}{u_i2^{i - k}} \right\rfloor \\
&= \sum_{i=k}^{n-1}{u_i2^{i - k}} 
= \sum_{i=0}^{n-k-1}{u_{i + k}2^{i}} 
\end{aligned}$$

算术右移, 其中  $k \in \{0, 1, \cdots, n-1\}$  :

$$\begin{aligned} 
x \gg_A k 
&= \left\lfloor x / 2^k \right\rfloor \\ 
&= \left\lfloor -u_{n-1}2^{n - k - 1} + \sum_{i=0}^{n-2}{u_i2^{i - k}} \right\rfloor \\
&= -u_{n-1}2^{n - k - 1} + \sum_{i=k}^{n-2}{u_i2^{i - k}} \\
&= -u_{n-1}2^{n - k} + \sum_{i=k}^{n-1}{u_i2^{i - k}} \\
&= -u_{n-1}2^{n - k} + \sum_{i=0}^{n-k-1}{u_{i + k}2^{i}} \\
&= u_{n-1} \left(-2^{n- 1} + \sum_{i=n-k}^{n-2}{2^{i}}\right) + \sum_{i=0}^{n-k-1}{u_{i + k}2^{i}} \\
\end{aligned}$$

上面推导借用了结论:  $\sum_{i=n}^{m} 2^{i} = 2^{m+1} - 2^{n}$ . 可见算术右移中符号位进行了扩展.

所以,  $x \gg_A k = u_{n-1} (-2^{n- 1} + \sum_{i=n-k}^{n-2}{2^{i}}) + x \gg_L k$.

特别地, 当  $x > 0$  时, 即当  $u_{n-1} = 0$  时,  $x \gg_A k = x \gg_L k$  .

在 C++ 14 之前

> For unsigned ` a ` and for signed and non-negative ` a ` , the value of ` a >> b ` is the integer part of  $a / 2^b$  .  For negative ` a ` , the value of ` a >> b ` is implementation-defined (in most implementations, this performs arithmetic right shift, so that the result remains negative).

在 C++ 14 之后

> The value of ` a >> b ` is  $a / 2^b$  , rounded down (in other words, right shift on signed ` a ` is arithmetic right shift).

***

### **更新记录**
- 20200722, 发布
  
### **版权声明**
版权声明: 自由分享, 保持署名-非商业用途-非衍生, 知识共享3.0协议.  
如果你对本文有疑问或建议, 欢迎留言! 转载请保留版权声明!

