#! https://www.zhihu.com/question/410906389/answer/1371814495

[comment]: <> (Answer URL: https://www.zhihu.com/question/410906389/answer/1371814495)
[comment]: <> (Question Title: （n-1）& x = x & (n -1) = x mod n 成立吗？如何证明？)
[comment]: <> (Author Name: 采石工)
[comment]: <> (Create Time: 2020-07-30 18:53:34)

令无符号数  $x = \sum\nolimits_{i = 0}^{m - 1} {{u_i}{2^i}}$,  $n = 2^k$, 其中 $u_i \in\left\{ 0, 1 \right\}$  且  $k \leq m$  .

$$n -1 = 2^k - 1 = \sum\nolimits_{i=0}^{k-1}2^i$$

$$\begin{aligned} 
x \& (n-1) 
&= \left( \sum\nolimits_{i = 0}^{m - 1}{{u_i}{2^i}} \right) \& \left( \sum\nolimits{i=0}^{k-1}2^i\right) \\
&= \sum\nolimits_{i=0}^{k-1}u_i2^i 
\end{aligned}$$

$$\begin{aligned} 
x \, \mathrm{mod} \, n 
&= x - \left[ x/n \right] \times n \\ 
&= \sum\nolimits_{i = 0}^{m - 1} {{u_i}{2^i}} - \left[\sum\nolimits_{i = 0}^{m - 1} {{u_i}{2^{i-k}}}\right]\times 2^k \\ 
&= \sum\nolimits_{i = 0}^{m - 1} {{u_i}{2^i}} - \left(\sum\nolimits_{i = k}^{m - 1} {{u_i}{2^{i-k}}}\right)\times 2^k \\ 
&= \sum\nolimits_{i = 0}^{m - 1} {{u_i}{2^i}} - \sum\nolimits_{i = k}^{m - 1} {{u_i}{2^{i}}} \\
&=\sum\nolimits_{i = 0}^{k - 1} {{u_i}{2^i}} 
\end{aligned}$$

上式中  $\left[\cdot\right]$  表示向零取整. 上述两式相等, 得证.

